Create a much simpler "base" representation of heaps

src/Heap.v
@@ -1,83 +1,26 @@
 Require Import
-  Fiat.ADT
-  Fiat.ADTNotation
-  ByteString.TupleEnsembles
-  ByteString.LibExt
-  ByteString.Nomega
-  ByteString.Decidable
-  ByteString.BindDep
-  ByteString.ADTInduction
-  ByteString.Same_set
-  ByteString.TupleEnsemblesFinite.
+  ByteString.Memory
+  ByteString.FMapExt
+  Coq.FSets.FMapFacts
+  Coq.Structures.DecidableTypeEx.
 
 Generalizable All Variables.
 
+Module Heap (M : WSfun N_as_DT).
+
+Module Import FMapExt := FMapExt N_as_DT M.
+Module P := FMapExt.P.
+Module F := P.F.
+
+Require Import
+  Fiat.ADT
+  Fiat.ADTNotation
+  ByteString.LibExt
+  ByteString.Nomega
+  ByteString.BindDep
+  ByteString.ADTInduction.
+
 Open Scope string_scope.
-
-Definition Word8 := Ascii.ascii.
-Definition Zero  := Ascii.zero.
-
-Record MemoryBlock := {
-  memSize : N;
-  memData : EMap N Word8
-}.
-
-Definition MemoryBlock_Same (x y : MemoryBlock) : Prop :=
-  memSize x = memSize y /\ Same (memData x) (memData y).
-
-Global Program Instance MemoryBlock_Proper :
-  Proper (eq ==> @Same _ _ ==> MemoryBlock_Same) Build_MemoryBlock.
-Obligation 1. relational; split; simpl; subst; auto. Qed.
-
-Ltac tsubst :=
-  repeat
-    match goal with
-    | [ H : (_, _) = (_, _) |- _ ] => inv H
-    | [ H : (_, _, _) = (_, _, _) |- _ ] => inv H
-    | [ H : (_, _, _, _) = (_, _, _, _) |- _ ] => inv H
-    | [ H : {| memSize := _
-             ; memData := _ |} =
-            {| memSize := _
-             ; memData := _ |} |- _ ] => inv H
-    end;
-  subst.
-
-Definition KeepKeys (P : N -> Prop) :
-  EMap N Word8 -> EMap N Word8 :=
-  Filter (fun k _ => P k).
-
-Definition ShiftKeys (orig_base : N) (new_base : N) :
-  EMap N Word8 -> EMap N Word8 :=
-  Map_set (fun p => (fst p - orig_base + new_base, snd p)).
-
-Definition FindFreeBlock (len : N) (heap : EMap N MemoryBlock) : Comp N :=
-  { addr : N | All (fun addr' blk' =>
-                      ~ overlaps addr' (memSize blk') addr len) heap }.
-
-Definition FindBlock (base : N) (heap : EMap N MemoryBlock) :
-  Comp (option MemoryBlock) :=
-  { blk : option MemoryBlock
-  | Ifopt blk as blk'
-    Then Lookup base blk' heap
-    Else ~ Member base heap }.
-
-Definition FindBlockThatFits (off len : N) (heap : EMap N MemoryBlock) :
-  Comp (option (N * MemoryBlock)) :=
-  { mres : option (N * MemoryBlock)
-  | match mres with
-    | Some (addr', blk') =>
-      Lookup addr' blk' heap /\ fits addr' (memSize blk') off len
-    | None =>
-      All (fun addr' blk' =>
-             ~ fits addr' (memSize blk') off len) heap
-    end }.
-
-Definition CopyBlock sblk soff dblk doff len :=
-  (* [s] is the source region to copy from *)
-  let s := KeepKeys (within soff len) (memData sblk) in
-  (* [d] is where the region will be copied *)
-  let d := KeepKeys (not ∘ within doff len) (memData dblk) in
-  Union _ d (ShiftKeys soff doff s).
 
 Definition emptyS   := "empty".
 Definition allocS   := "alloc".
@@ -88,12 +31,129 @@ Definition pokeS    := "poke".
 Definition memcpyS  := "memcpy".
 Definition memsetS  := "memset".
 
+Record HeapState := {
+  resvs : M.t Size;
+  bytes : M.t Word
+}.
+
+Definition newHeapState :=
+  {| resvs := M.empty _
+   ; bytes := M.empty _ |}.
+
+Definition find_free_block (len : Size) (r : M.t Ptr) : Comp Ptr :=
+  { addr : N | P.for_all (fun a sz => negb (overlaps_bool a sz addr len)) r }.
+
+Definition keep_keys (P : M.key -> bool) : M.t Word -> M.t Word :=
+  P.filter (const ∘ P).
+
+Definition keep_range (addr : Ptr) (len : Size) : M.t Word -> M.t Word :=
+  keep_keys (within_bool addr len).
+
+Definition drop_range (addr : Ptr) (len : Size) : M.t Word -> M.t Word :=
+  keep_keys (fun p => negb (within_bool addr len p)).
+
+Definition shift_keys (orig_base : N) (new_base : N) (m : M.t Word) :
+  M.t Word :=
+  M.fold (fun k e rest =>
+            If orig_base <=? k
+            Then M.add (k - orig_base + new_base) e rest
+            Else rest) m (M.empty _).
+
+Definition copy_bytes (from to len : Ptr) (bytes : M.t Word) : M.t Word :=
+  P.update (drop_range to len bytes)
+           (shift_keys from to (keep_range from len bytes)).
+
+Program Instance copy_bytes_Proper :
+  Proper (eq ==> eq ==> eq ==> M.Equal ==> M.Equal) copy_bytes.
+Obligation 1.
+  relational.
+  unfold copy_bytes, drop_range, keep_range, shift_keys, keep_keys.
+  apply P.update_m; trivial.
+    rewrite H2; reflexivity.
+  apply P.fold_Equal; eauto; relational.
+  - destruct (y <=? y3); simpl.
+      rewrite H1; reflexivity.
+    assumption.
+  - intros ??????.
+    destruct (y <=? k) eqn:Heqe; simpl;
+    destruct (y <=? k') eqn:Heqe1; simpl;
+    try reflexivity.
+    rewrite add_associative.
+      reflexivity.
+    intros.
+    apply N.add_cancel_r in H0.
+    apply Nsub_eq in H0; try tauto; nomega.
+  - rewrite H2; reflexivity.
+Qed.
+
+Lemma copy_bytes_idem d len m : M.Equal (copy_bytes d d len m) m.
+Proof.
+  unfold copy_bytes, drop_range, keep_range,
+         shift_keys, keep_keys, const, not, compose.
+  apply F.Equal_mapsto_iff; split; intros.
+    apply P.update_mapsto_iff in H.
+    destruct H.
+      revert H.
+      apply P.fold_rec_bis; simpl; intros; intuition.
+      destruct (d <=? k0); simpl in *.
+        do 2 simplify_maps; relational.
+        rewrite N.sub_add; trivial.
+        nomega.
+      intuition.
+    destruct H.
+    simplify_maps; relational.
+  apply P.update_mapsto_iff.
+  destruct (within_bool d len k) eqn:Heqe.
+    left.
+    remember (fun _ _ => within_bool _ _ _) as f.
+    assert (Proper (eq ==> eq ==> eq) f) by relational.
+    rewrite Heqf in H0.
+    simpl in H0.
+    assert ((fun H _ => within_bool d len H) k e = true).
+      nomega.
+    pose proof (proj2 (P.filter_iff H0 m k e) (conj H H1)).
+    revert H2.
+    rewrite <- Heqf.
+    apply P.fold_rec_bis; simpl; intros; intuition.
+      rewrite <- H2 in H4.
+      intuition.
+    destruct (d <=? k0) eqn:Heqe1; simpl.
+      rewrite N.sub_add; trivial.
+        simplify_maps.
+          do 2 simplify_maps.
+        simplify_maps; relational.
+        simplify_maps; relational.
+      nomega.
+    apply H4.
+    simplify_maps.
+    nomega.
+  right.
+  split.
+    simplify_maps; relational.
+    split; trivial.
+    nomega.
+  apply P.fold_rec_bis; simpl; intros; intuition.
+    inversion H0.
+    simplify_maps.
+  destruct (d <=? k0) eqn:Heqe1; simpl in H3.
+    apply (proj1 (in_mapsto_iff _ _ _)) in H3.
+    destruct H3.
+    simplify_maps.
+      simplify_maps; relational.
+      nomega.
+    contradiction H2.
+    apply in_mapsto_iff.
+    exists x.
+    assumption.
+  contradiction.
+Qed.
+
 Definition HeapSpec := Def ADT {
   (* Map of memory addresses to blocks, which contain another mapping from
      offsets to initialized bytes. *)
-  rep := EMap N MemoryBlock,
+  rep := HeapState,
 
-  Def Constructor0 emptyS : rep := ret Empty,,
+  Def Constructor0 emptyS : rep := ret newHeapState,,
 
   (* Allocation returns the address for the newly allocated block.
      NOTE: conditions such as out-of-memory are not handled here; the final
@@ -102,109 +162,86 @@ Definition HeapSpec := Def ADT {
      specify error handling at this level, when certain errors -- such as
      exhausting memory -- do not belong here, since a mathematical machine has
      no such limits. *)
-  Def Method1 allocS (r : rep) (len : N | 0 < len) : rep * N :=
-    addr <- FindFreeBlock (` len) r;
-    ret (Update addr {| memSize := ` len
-                      ; memData := Empty |} r, addr),
+  Def Method1 allocS (r : rep) (len : Size | 0 < len) : rep * Ptr :=
+    addr <- find_free_block (` len) (resvs r);
+    ret ({| resvs := M.add addr (` len) (resvs r)
+          ; bytes := bytes r |}, addr),
 
   (* Freeing an unallocated block is a no-op. *)
-  Def Method1 freeS (r : rep) (addr : N) : rep * unit :=
-    ret (Remove addr r, tt),
+  Def Method1 freeS (r : rep) (addr : Ptr) : rep * unit :=
+    ret ({| resvs := M.remove addr (resvs r)
+          ; bytes := bytes r |}, tt),
 
   (* Realloc is not required to reuse the same block. If the address does not
      identify an allociated region, a new memory block is returned without any
      bytes moved. If a block did exist previously, as many bytes as possible
      are copied to the new block. *)
-  Def Method2 reallocS (r : rep) (addr : N) (len : N | 0 < len) : rep * N :=
-    present <- FindBlock addr r;
-    naddr   <- FindFreeBlock (` len) (Remove addr r);
-    ret (
-      Ifopt present as blk
-      Then Update naddr {| memSize := ` len
-                         ; memData := Filter (fun pos _ => pos < ` len)
-                                             (memData blk) |} (Remove addr r)
-      Else Update naddr {| memSize := ` len
-                         ; memData := Empty |} r,
-      naddr),
+  Def Method2 reallocS (r : rep) (addr : Ptr) (len : Size | 0 < len) :
+    rep * Ptr :=
+    naddr <- find_free_block (` len) (M.remove addr (resvs r));
+    ret ({| resvs := M.add naddr (` len) (M.remove addr (resvs r))
+          ; bytes :=
+              Ifopt M.find addr (resvs r) as sz
+              Then copy_bytes addr naddr (N.min sz (` len)) (bytes r)
+              Else bytes r |}, naddr),
 
-  (* Peeking an unallocated address allows anydefault value to be returned. *)
-  Def Method1 peekS (r : rep) (addr : N) : rep * Word8 :=
-    mres <- FindBlockThatFits addr 1 r;
-    p <- { p : Word8
-         | forall v base' blk', mres = Some (base', blk')
-             -> Lookup (addr - base') v (memData blk')
-             -> p = v };
+  (* Peeking an uninitialized address allows any value to be returned. *)
+  Def Method1 peekS (r : rep) (addr : Ptr) : rep * Word :=
+    p <- { p : Word | forall v, M.MapsTo addr v (bytes r) -> p = v };
     ret (r, p),
 
-  (* Poking an unallocated address is a no-op. *)
-  Def Method2 pokeS (r : rep) (addr : N) (w : Word8) : rep * unit :=
-    ret (Map (fun base blk =>
-                Ifdec within base (memSize blk) addr
-                Then {| memSize := memSize blk
-                      ; memData := Update (addr - base) w (memData blk) |}
-                Else blk) r, tt),
+  Def Method2 pokeS (r : rep) (addr : Ptr) (w : Word) : rep * unit :=
+    ret ({| resvs := resvs r
+          ; bytes := M.add addr w (bytes r) |}, tt),
 
   (* Data may only be copied from one allocated block to another (or within
      the same block), and the region must fit within both source and
      destination. Otherwise, the operation is a no-op. *)
-  Def Method3 memcpyS (r : rep) (addr1 : N) (addr2 : N) (len : N) :
+  Def Method3 memcpyS (r : rep) (addr1 : Ptr) (addr2 : Ptr) (len : Size) :
     rep * unit :=
-      Ifdec 0 < len
-      Then (
-        ms <- FindBlockThatFits addr1 len r;
-        ret (Ifopt ms as s
-             Then
-               Map (fun daddr dblk =>
-                 Ifdec fits daddr (memSize dblk) addr2 len
-                 Then {| memSize := memSize dblk
-                       ; memData :=
-                           let soff := addr1 - fst s in
-                           let doff := addr2 - daddr in
-                           CopyBlock (snd s) soff dblk doff len |}
-                 Else dblk) r
-             Else r, tt))
-      Else ret (r, tt),
+    ret ({| resvs := resvs r
+          ; bytes := copy_bytes addr1 addr2 len (bytes r) |}, tt),
 
   (* Any attempt to memset bytes outside of an allocated block is a no-op. *)
-  Def Method3 memsetS (r : rep) (addr : N) (len : N) (w : Word8) :
+  Def Method3 memsetS (r : rep) (addr : Ptr) (len : Size) (w : Word) :
     rep * unit :=
-    ret (Map (fun base blk =>
-                Ifdec fits base (memSize blk) addr len
-                Then {| memSize := memSize blk
-                      ; memData := Define (within (addr - base) len) w
-                                          (memData blk) |}
-                Else blk) r, tt)
+    ret ({| resvs := resvs r
+          ; bytes :=
+              P.update (bytes r)
+                       (N.peano_rect (fun _ => M.t Word) (bytes r)
+                                     (fun i => M.add (addr + i)%N w)
+                                     len) |}, tt)
 
 }%ADTParsing.
 
 Definition empty : Comp (Rep HeapSpec) :=
   Eval simpl in callCons HeapSpec emptyS.
 
-Definition alloc (r : Rep HeapSpec) (len : N | 0 < len) :
+Definition alloc (r : Rep HeapSpec) (len : Size | 0 < len) :
   Comp (Rep HeapSpec * N) :=
   Eval simpl in callMeth HeapSpec allocS r len.
 
-Definition free (r : Rep HeapSpec) (addr : N) :
+Definition free (r : Rep HeapSpec) (addr : Ptr) :
   Comp (Rep HeapSpec * unit) :=
   Eval simpl in callMeth HeapSpec freeS r addr.
 
-Definition realloc (r : Rep HeapSpec) (addr : N) (len : N | 0 < len) :
+Definition realloc (r : Rep HeapSpec) (addr : Ptr) (len : Size | 0 < len) :
   Comp (Rep HeapSpec * N) :=
   Eval simpl in callMeth HeapSpec reallocS r addr len.
 
-Definition peek (r : Rep HeapSpec) (addr : N) :
-  Comp (Rep HeapSpec * Word8) :=
+Definition peek (r : Rep HeapSpec) (addr : Ptr) :
+  Comp (Rep HeapSpec * Word) :=
   Eval simpl in callMeth HeapSpec peekS r addr.
 
-Definition poke (r : Rep HeapSpec) (addr : N) (w : Word8) :
+Definition poke (r : Rep HeapSpec) (addr : Ptr) (w : Word) :
   Comp (Rep HeapSpec * unit) :=
   Eval simpl in callMeth HeapSpec pokeS r addr w.
 
-Definition memcpy (r : Rep HeapSpec) (addr : N) (addr2 : N) (len : N) :
+Definition memcpy (r : Rep HeapSpec) (addr : Ptr) (addr2 : Ptr) (len : Size) :
   Comp (Rep HeapSpec * unit) :=
   Eval simpl in callMeth HeapSpec memcpyS r addr addr2 len.
 
-Definition memset (r : Rep HeapSpec) (addr : N) (len : N) (w : Word8) :
+Definition memset (r : Rep HeapSpec) (addr : Ptr) (len : Ptr) (w : Word) :
   Comp (Rep HeapSpec * unit) :=
   Eval simpl in callMeth HeapSpec memsetS r addr len w.
 
@@ -213,12 +250,15 @@ Definition memset (r : Rep HeapSpec) (addr : N) (len : N) (w : Word8) :
  **)
 
 Ltac inspect :=
-  repeat (unfold KeepKeys, ShiftKeys, CopyBlock,
-                 FindFreeBlock, FindBlock, FindBlockThatFits in *;
+  unfold find_free_block, copy_bytes,
+         keep_keys, shift_keys, newHeapState in *;
+  destruct_computations; simpl in *;
+  repeat breakdown;
+  repeat (simplify_maps; simpl in *;
+          unfold find_free_block, copy_bytes,
+                 keep_keys, shift_keys, newHeapState in *;
           destruct_computations; simpl in *;
-          repeat teardown; tsubst; simpl in *;
-          decisions; eauto with sets;
-          try congruence).
+          repeat breakdown).
 
 Ltac complete IHfromADT :=
   inspect;
@@ -234,213 +274,607 @@ Ltac complete IHfromADT :=
             | discriminate ].
 
 Theorem allocations_have_size : forall r : Rep HeapSpec, fromADT _ r ->
-  forall addr blk, Lookup addr blk r -> 0 < memSize blk.
+  forall addr sz, M.MapsTo addr sz (resvs r) -> 0 < sz.
 Proof.
   intros.
-  generalize dependent blk.
+  generalize dependent sz.
   generalize dependent addr.
-  ADT induction r; [inversion H0|..]; complete IHfromADT.
+  ADT induction r; complete IHfromADT.
 Qed.
 
-Theorem allocations_correct_offsets : forall r : Rep HeapSpec, fromADT _ r ->
-  forall addr blk, Lookup addr blk r ->
-    All (fun off _ => off < memSize blk) (memData blk).
-Proof.
-  intros.
-  generalize dependent blk.
-  generalize dependent addr.
-  ADT induction r; [inversion H0|..]; intros ???;
-  complete IHfromADT.
-Qed.
+Definition does_not_overlap addr len :=
+  fun a sz => negb (overlaps_bool a sz addr len).
 
-Ltac match_sizes H IHfromADT :=
-  match goal with
-  | [ H1 : Lookup ?A ?X ?R, H2 : Lookup ?B ?Y ?R |- _ ] =>
-    specialize (IHfromADT _ _
-                  H1 (allocations_have_size H _ _ H1) _
-                  H2 (allocations_have_size H _ _ H2)); subst
-  end; inspect; auto.
+Corollary negb_overlaps_bool_Proper addr len :
+  Proper (eq ==> eq ==> eq) (does_not_overlap addr len).
+Proof. relational. Qed.
 
-Ltac match_sizes_r H IHfromADT :=
+Ltac apply_for_all :=
+  try match goal with
+  | [ H1 : is_true (P.for_all ?P ?m),
+      H2 : M.MapsTo ?k ?e ?m |- _ ] => unfold is_true in H1
+  end;
   match goal with
-  | [ H1 : Lookup ?A ?X ?R, H2 : Lookup ?B ?Y ?R |- _ ] =>
-    try rewrite <- (IHfromADT _ _
-                      H1 (allocations_have_size H _ _ H1) _
-                      H2 (allocations_have_size H _ _ H2)) in *
-  end; inspect; auto.
-
-Ltac check_overlaps :=
-  match goal with
-    [ H1 : All (fun addr' blk' => ~ overlaps addr' (memSize blk') ?XA ?XL)
-               (Remove ?YA ?R),
-      H2 : ?XA <> ?YA,
-      H3 : 0 < ?XL,
-      H4 : Lookup ?XA ?B ?R,
-      H5 : 0 < memSize ?B |- _ ] =>
-    eapply All_Remove_Lookup_inv with (a':=XA) in H1; eauto;
-    contradiction (overlaps_irr XA H5 H3)
+  | [ H1 : P.for_all ?P ?m = true,
+      H2 : M.MapsTo ?k ?e ?m |- _ ] =>
+    cut (Proper (eq ==> eq ==> eq) P);
+    [ let HP := fresh "HP" in
+      intro HP;
+      let H := fresh "H" in
+      pose proof (proj1 (@P.for_all_iff _ P HP m) H1 k e H2) as H;
+      simpl in H | ]
   end.
 
-Theorem allocations_functional : forall r : Rep HeapSpec, fromADT _ r ->
-  Functional r.
-Proof.
-  unfold Functional; intros.
-  pose proof (allocations_have_size H _ _ H0).
-  pose proof (allocations_have_size H _ _ H1).
-  generalize dependent blk2.
-  generalize dependent blk1.
-  generalize dependent addr.
-  ADT induction r; [inversion H0|..]; inspect;
-  try solve [ match_sizes H IHfromADT ];
-  try discriminate;
-  check_overlaps.
-Qed.
-
-Theorem all_block_maps_are_functional : forall r : Rep HeapSpec, fromADT _ r ->
-  All (fun _ blk => Functional (memData blk)) r.
-Proof.
-  unfold All, Functional; intros.
-  generalize dependent b.
-  generalize dependent a.
-  generalize dependent blk1.
-  generalize dependent blk2.
-  generalize dependent addr.
-  ADT induction r; inspect.
-  - unfold compose in *; nomega.
-  - unfold compose in *; nomega.
-  - apply N.add_cancel_r in H9.
-    apply Nsub_eq in H9.
-    + subst.
-      clear H4.
-      eapply IHfromADT; eauto.
-    + nomega.
-    + nomega.
-  - inv H3; inv H4; congruence.
-Qed.
-
-Corollary allocations_functional_r : forall r : Rep HeapSpec, fromADT _ r ->
-  forall addr1 blk, Lookup addr1 blk r ->
-  forall addr2, ~ Member addr2 r -> addr1 <> addr2.
-Proof.
-  unfold not; intros; subst; ADT induction r;
-  contradiction H1;
-  exists blk; assumption.
-Qed.
-
-Ltac lookup_uid H :=
-  match goal with
-  | [ H1 : Lookup ?A ?X ?R, H2 : Lookup ?A ?Y ?R |- _ ] =>
-    pose proof (allocations_functional H _ _ H1 _ H2); subst
-  end; inspect; auto.
-
 Theorem allocations_no_overlap : forall r : Rep HeapSpec, fromADT _ r ->
-  forall addr1 blk1, Lookup addr1 blk1 r ->
-  forall addr2 blk2, Lookup addr2 blk2 r
+  forall addr1 sz1, M.MapsTo addr1 sz1 (resvs r) ->
+  forall addr2 sz2, M.MapsTo addr2 sz2 (resvs r)
     -> addr1 <> addr2
-    -> ~ overlaps addr1 (memSize blk1) addr2 (memSize blk2).
+    -> ~ overlaps addr1 sz1 addr2 sz2.
 Proof.
   intros.
-  pose proof (allocations_have_size H _ _ H0).
-  pose proof (allocations_have_size H _ _ H1).
-  generalize dependent blk2.
+  pose proof (allocations_have_size H H0).
+  pose proof (allocations_have_size H H1).
+  generalize dependent sz2.
   generalize dependent addr2.
-  generalize dependent blk1.
+  generalize dependent sz1.
   generalize dependent addr1.
-  ADT induction r; [inversion H0|..]; complete IHfromADT;
-  try lookup_uid H; eapply All_Remove_Lookup_inv in H0'; eauto;
-  try nomega; eapply allocations_functional_r in H0; eauto.
+  ADT induction r; complete IHfromADT.
+  - apply_for_all; nomega.
+  - apply_for_all; nomega.
+  - eapply M.remove_2 in H4; eauto.
+    apply_for_all; nomega.
+  - clear H8.
+    eapply M.remove_2 in H4; eauto.
+    apply not_overlaps_sym.
+    apply_for_all; nomega.
 Qed.
+
+Theorem allocations_no_overlap_r : forall r : Rep HeapSpec, fromADT _ r ->
+  forall addr1 sz1,
+    P.for_all (fun a sz => negb (overlaps_bool a sz addr1 sz1)) (resvs r)
+      -> 0 < sz1
+      -> ~ M.In addr1 (resvs r).
+Proof.
+  unfold not; intros.
+  generalize dependent sz1.
+  generalize dependent addr1.
+  ADT induction r; complete IHfromADT.
+  - inversion H2.
+    simplify_maps.
+  - apply (proj1 (in_mapsto_iff _ _ _)) in H2.
+    destruct H2.
+    apply for_all_add_true in H1;
+    relational; simpl in *.
+      simplify_maps.
+        nomega.
+      assert (M.In addr1 (resvs r)).
+        apply in_mapsto_iff.
+        exists x1; assumption.
+      eapply IHfromADT; eauto.
+      nomega.
+    unfold not; intros.
+    eapply IHfromADT; eauto.
+  - apply (proj1 (in_mapsto_iff _ _ _)) in H2.
+    destruct H2.
+    simplify_maps.
+    eapply for_all_remove_inv in H1; relational.
+      eapply IHfromADT; eauto.
+      apply in_mapsto_iff.
+      exists x0; assumption.
+    unfold not; intros.
+    apply (proj1 (in_mapsto_iff _ _ _)) in H0.
+    destruct H0.
+    pose proof (allocations_have_size H H4).
+    apply not_eq_sym in H2.
+    eapply F.remove_neq_mapsto_iff in H4; eauto.
+    apply_for_all; relational.
+    nomega.
+  - apply (proj1 (in_mapsto_iff _ _ _)) in H2.
+    destruct H2.
+    simpl in *.
+    apply_for_all; relational.
+    rewrite <- remove_add in H1.
+    simplify_maps.
+      apply for_all_add_true in H1; relational; simpl in *.
+        nomega.
+      simplify_maps.
+    rewrite remove_add in H1.
+    apply_for_all; relational.
+    simplify_maps.
+    pose proof (allocations_have_size H H6).
+    nomega.
+Qed.
+
+Definition unique {A : Type} (P : M.key -> A -> bool) a r :=
+  P.for_all (fun a b => negb (P a b)) (M.remove a r).
+
+Corollary negb_fits_bool_Proper addr len :
+  Proper (eq ==> eq ==> eq) (fun a b => negb (fits_bool a b addr len)).
+Proof. relational. Qed.
 
 Corollary allocations_unique_fits : forall r : Rep HeapSpec, fromADT _ r ->
-  forall base blk addr len,
-    Lookup base blk r ->
-    fits base (memSize blk) addr len ->
-    Unique (fun a' b' => fits_bool a' (memSize b') addr len) base r.
+  forall base sz addr len,
+    M.MapsTo base sz (resvs r) ->
+    fits base sz addr len ->
+    unique (fun a' b' => fits_bool a' b' addr len) base (resvs r).
 Proof.
-  unfold Unique; intros; intros ???.
-  apply Lookup_Remove_inv in H2; destruct H2.
-  pose proof (allocations_no_overlap H _ H3 _ H0 H2); nomega.
+  unfold unique; intros.
+  apply P.for_all_iff; intros.
+    apply negb_fits_bool_Proper.
+  simplify_maps.
+  pose proof (allocations_no_overlap H H0 H4 H3); nomega.
 Qed.
 
+Corollary within_bool_Proper addr :
+  Proper (eq ==> eq ==> eq) (fun a b => within_bool a b addr).
+Proof. relational. Qed.
+
+Corollary negb_within_bool_Proper addr :
+  Proper (eq ==> eq ==> eq) (fun a b => negb (within_bool a b addr)).
+Proof. relational. Qed.
+
 Corollary allocations_unique_within : forall r : Rep HeapSpec, fromADT _ r ->
-  forall base blk addr,
-    Lookup base blk r ->
-    within base (memSize blk) addr ->
-    Unique (fun a' b' => within_bool a' (memSize b') addr) base r.
+  forall base sz addr,
+    M.MapsTo base sz (resvs r) ->
+    within base sz addr ->
+    unique (fun a' b' => within_bool a' b' addr) base (resvs r).
 Proof.
-  unfold Unique; intros; intros ???.
-  apply Lookup_Remove_inv in H2; destruct H2.
-  pose proof (allocations_no_overlap H _ H3 _ H0 H2); nomega.
+  unfold unique; intros.
+  apply P.for_all_iff; intros.
+    apply negb_within_bool_Proper.
+  simplify_maps.
+  pose proof (allocations_no_overlap H H0 H4 H3); nomega.
 Qed.
 
 Corollary find_partitions_a_singleton : forall r : Rep HeapSpec, fromADT _ r ->
-  forall addr base blk,
-    Lookup base blk r
-      -> within base (memSize blk) addr
-      -> Same (Filter (fun a b => within a (memSize b) addr) r)
-              (Single base blk).
+  forall addr base sz,
+    M.MapsTo base sz (resvs r)
+      -> within base sz addr
+      -> M.Equal (P.filter (fun a b => within_bool a b addr) (resvs r))
+                 (singleton base sz).
 Proof.
   intros.
-  pose proof (allocations_no_overlap H _ H0).
-  pose proof (allocations_functional H _ _ H0).
-  split; intros; inspect;
-  destruct (N.eq_dec base a); subst; auto.
-  - specialize (H2 _ _ H5 n); nomega.
-  - specialize (H3 _ H5); nomega.
-  - specialize (H2 _ _ H5 n); nomega.
+  pose proof (allocations_no_overlap H H0).
+  apply F.Equal_mapsto_iff; intros.
+  split; intros.
+    unfold singleton.
+    simplify_maps.
+      simplify_maps.
+      destruct (N.eq_dec base k); subst.
+        pose proof (F.MapsTo_fun H4 H0); subst.
+        left; intuition.
+      right; intuition.
+      specialize (H2 _ _ H4 n).
+      contradiction H2.
+      nomega.
+    apply within_bool_Proper.
+  unfold singleton in H3.
+  simplify_maps.
+  simplify_maps.
+    apply within_bool_Proper.
+  intuition; nomega.
 Qed.
 
 Corollary allocations_disjoint : forall r : Rep HeapSpec, fromADT _ r ->
-  forall addr blk, Lookup addr blk r
-    -> forall pos, within addr (memSize blk) pos
-    -> forall addr' blk', Lookup addr' blk' r
+  forall addr sz, M.MapsTo addr sz (resvs r)
+    -> forall pos, within addr sz pos
+    -> forall addr' sz', M.MapsTo addr' sz' (resvs r)
          -> addr <> addr'
-         -> ~ within addr' (memSize blk') pos.
-Proof. intros; pose proof (allocations_no_overlap H _ H0 _ H2 H3); nomega. Qed.
+         -> ~ within addr' sz' pos.
+Proof. intros; pose proof (allocations_no_overlap H H0 H2 H3); nomega. Qed.
 
-Theorem heap_is_finite : forall r : Rep HeapSpec, fromADT _ r -> Finite _ r.
-Proof. intros; ADT induction r; inspect; finite_preservation; nomega. Qed.
+End Heap.
 
-Lemma added : forall b e,
-  b <= e -> Same_set _ (fun x : N => b <= x < N.succ e)
-                       (Add _ (fun x : N => b <= x < e) e).
+Module HeapADT (M : WSfun N_as_DT).
+
+Module Import Heap := Heap M.
+
+Require Import
+  Coq.NArith.NArith
+  Fiat.ADT
+  Fiat.ADTNotation
+  ByteString.ADTInduction
+  ByteString.FromADT.
+
+Open Scope N_scope.
+
+Lemma empty_fromADT r :
+  refine (callCons HeapSpec emptyS) (ret r) -> fromADT HeapSpec r.
+Proof. check constructor (fromCons HeapSpec emptyS r). Qed.
+
+Lemma alloc_fromADT r :
+  fromADT HeapSpec r
+    -> forall (len : Size | 0 < len) v,
+         refine (callMeth HeapSpec allocS r len) (ret v)
+    -> fromADT HeapSpec (fst v).
+Proof. intros; check method (fromMeth HeapSpec allocS r (fst v)). Qed.
+
+Lemma free_fromADT r :
+  fromADT HeapSpec r
+    -> forall (addr : Ptr) v,
+         refine (callMeth HeapSpec freeS r addr) (ret v)
+    -> fromADT HeapSpec (fst v).
+Proof. intros; check method (fromMeth HeapSpec freeS r (fst v)). Qed.
+
+Lemma realloc_fromADT r :
+  fromADT HeapSpec r
+    -> forall (addr : Ptr) (len : Size | 0 < len) v,
+         refine (callMeth HeapSpec reallocS r addr len) (ret v)
+    -> fromADT HeapSpec (fst v).
+Proof. intros; check method (fromMeth HeapSpec reallocS r (fst v)). Qed.
+
+Lemma peek_fromADT r :
+  fromADT HeapSpec r
+    -> forall (addr : Ptr) v,
+         refine (callMeth HeapSpec peekS r addr) (ret v)
+    -> fromADT HeapSpec (fst v).
+Proof. intros; check method (fromMeth HeapSpec peekS r (fst v)). Qed.
+
+Lemma poke_fromADT r :
+  fromADT HeapSpec r
+    -> forall (addr : Ptr) w v,
+         refine (callMeth HeapSpec pokeS r addr w) (ret v)
+    -> fromADT HeapSpec (fst v).
+Proof. intros; check method (fromMeth HeapSpec pokeS r (fst v)). Qed.
+
+Lemma memcpy_fromADT r :
+  fromADT HeapSpec r
+    -> forall (addr : Ptr) (addr2 : Ptr) (len : Size) v,
+         refine (callMeth HeapSpec memcpyS r addr addr2 len) (ret v)
+    -> fromADT HeapSpec (fst v).
+Proof. intros; check method (fromMeth HeapSpec memcpyS r (fst v)). Qed.
+
+Lemma memset_fromADT r :
+  fromADT HeapSpec r
+    -> forall (addr : Ptr) (len : Size) (w : Word) v,
+         refine (callMeth HeapSpec memsetS r addr len w) (ret v)
+    -> fromADT HeapSpec (fst v).
+Proof. intros; check method (fromMeth HeapSpec memsetS r (fst v)). Qed.
+
+Require Import
+  Fiat.ADTRefinement
+  Fiat.ADTRefinement.BuildADTRefinements.
+
+Theorem HeapSpecADT : { adt : _ & refineADT HeapSpec adt }.
 Proof.
-  unfold Same_set, Included, Add, Ensembles.In.
-  split; intros.
-    destruct (N.eq_dec x e); subst.
-      right; constructor.
-    left; unfold Ensembles.In in *; nomega.
-  inv H0; unfold Ensembles.In in *;
-  destruct H1; nomega.
-Qed.
+  eexists.
+  hone representation using
+    (fun (or : Rep HeapSpec)
+         (nr : { r : Rep HeapSpec | fromADT HeapSpec r }) => or = ` nr).
+  resolve_constructor empty empty_fromADT.
+  resolve_method r_n (alloc (` r_n) d)
+                     (@alloc_fromADT _ (proj2_sig r_n) d).
+  resolve_method r_n (free (` r_n) d)
+                     (@free_fromADT _ (proj2_sig r_n) d).
+  resolve_method r_n (realloc (` r_n) d d0)
+                     (@realloc_fromADT _ (proj2_sig r_n) d d0).
+  resolve_method r_n (peek (` r_n) d)
+                     (@peek_fromADT _ (proj2_sig r_n) d).
+  resolve_method r_n (poke (` r_n) d d0)
+                     (@poke_fromADT _ (proj2_sig r_n) d d0).
+  resolve_method r_n (memcpy (` r_n) d d0 d1)
+                     (@memcpy_fromADT _ (proj2_sig r_n) d d0 d1).
+  resolve_method r_n (memset (` r_n) d d0 d1)
+                     (@memset_fromADT _ (proj2_sig r_n) d d0 d1).
+  apply reflexivityT.
+Defined.
 
-Lemma not_added : forall b e,
-  ~ b <= e -> Same_set _ (fun x : N => b <= x < N.succ e)
-                         (fun x : N => b <= x < e).
-Proof. unfold Same_set, Included, Add, Ensembles.In; nomega. Qed.
+End HeapADT.
 
-Lemma N_Finite : forall b e, Finite N (fun x : N => b <= x < e).
+Module HeapCanonical (M : WSfun N_as_DT).
+
+Module Import HeapADT := HeapADT M.
+Import Heap.
+Import Heap.FMapExt.
+Module P := FMapExt.P.
+Module F := P.F.
+
+Require Import
+  Coq.NArith.NArith
+  Fiat.ADT
+  Fiat.ADTNotation
+  Fiat.ADTRefinement
+  Fiat.ADTRefinement.BuildADTRefinements
+  ByteString.ADTInduction
+  ByteString.FromADT
+  ByteString.BindDep
+  ByteString.Nomega
+  ByteString.Tactics.
+
+Open Scope N_scope.
+
+Definition within_allocated_mem (n : Ptr) :=
+  fun (addr : M.key) (sz : Size) => addr + sz <=? n.
+Arguments within_allocated_mem n addr sz /.
+
+(** In order to refine to a computable heap, we have to add the notion of
+    "free memory", from which addresses may be allocated. A further
+    optimization here would be to add a free list, to which free blocks are
+    returned, in order avoid gaps in the heap. A yet further optimization
+    would be to better manage the free space to avoid fragmentation. The
+    implementation below simply grows the heap with every allocation. *)
+
+Lemma HeapCanonical : FullySharpened HeapSpec.
 Proof.
-  intros.
-  induction e using N.peano_ind; intros.
-    eapply Finite_downward_closed; eauto with sets.
-    unfold Included, Ensembles.In; nomega.
-  destruct (N.le_decidable b e).
-    rewrite added; trivial.
-    constructor; trivial.
-    unfold Ensembles.In; nomega.
-  rewrite not_added; trivial.
-Qed.
+  start sharpening ADT.
+  eapply SharpenStep; [ apply (projT2 HeapSpecADT) |].
 
-Hint Extern 5 (Finite N (within _ _)) => apply N_Finite.
+  hone representation using
+       (fun or nr =>
+          M.Equal (resvs (` or)) (resvs (snd nr)) /\
+          M.Equal (bytes (` or)) (bytes (snd nr)) /\
+          P.for_all (within_allocated_mem (fst nr)) (resvs (snd nr))).
 
-Theorem all_blocks_are_finite : forall r : Rep HeapSpec, fromADT _ r ->
-  All (fun _ blk => Finite _ (memData blk)) r.
-Proof.
-  unfold All; intros.
-  generalize dependent b.
-  generalize dependent a.
-  ADT induction r; inspect;
-  finite_preservation;
-  eauto; nomega.
-Qed.
+  refine method emptyS.
+  {
+    remove_dependency.
+    simplify with monad laws.
+    refine pick val (0%N, newHeapState).
+      finish honing.
+    intuition; simpl.
+    apply for_all_empty; relational.
+  }
+
+  refine method allocS.
+  {
+    remove_dependency.
+    unfold alloc, find_free_block.
+    simplify with monad laws; simpl.
+
+    refine pick val (fst r_n).
+    {
+      simplify with monad laws; simpl.
+
+      refine pick val (fst r_n + ` d,
+                       {| resvs := M.add (fst r_n) (` d) (resvs (snd r_n))
+                        ; bytes := bytes (snd r_n) |}).
+        simplify with monad laws; simpl.
+        finish honing.
+
+      simpl in *; intuition.
+      rewrite H1; reflexivity.
+      apply for_all_add_true; relational.
+        rewrite <- H1.
+        destruct d.
+        eapply allocations_no_overlap_r; eauto.
+          exact (proj2_sig r_o).
+        rewrite H1.
+        eapply for_all_impl; eauto; relational; intros.
+        unfold within_allocated_mem in H2.
+        nomega.
+      split.
+        eapply for_all_impl; eauto; relational; intros.
+        unfold within_allocated_mem in *.
+        nomega.
+      nomega.
+    }
+
+    repeat breakdown; simpl in *.
+    rewrite H0.
+    eapply for_all_impl; eauto;
+    relational; nomega.
+  }
+
+  refine method freeS.
+  {
+    remove_dependency.
+    unfold free.
+    simplify with monad laws; simpl.
+
+    refine pick val (fst r_n,
+                     {| resvs := M.remove d (resvs (snd r_n))
+                      ; bytes := bytes (snd r_n) |}).
+      simplify with monad laws; simpl.
+      finish honing.
+
+    simpl in *; intuition.
+    - rewrite H1; reflexivity.
+    - apply for_all_remove; relational.
+  }
+
+  refine method reallocS.
+  {
+    remove_dependency.
+    unfold realloc, find_free_block.
+    simplify with monad laws; simpl.
+
+    refine pick val (Ifopt M.find d (resvs (snd r_n)) as sz
+                     Then If ` d0 <=? sz Then d Else fst r_n
+                     Else fst r_n).
+    {
+      simplify with monad laws.
+
+      refine pick val
+        (Ifopt M.find d (resvs (snd r_n)) as sz
+         Then If ` d0 <=? sz
+              Then
+                (fst r_n,
+                 {| resvs := M.add d (` d0) (resvs (snd r_n)) (* update *)
+                  ; bytes := bytes (snd r_n) |})
+              Else
+                (fst r_n + ` d0,
+                 {| resvs := M.add (fst r_n) (` d0)
+                                   (M.remove d (resvs (snd r_n)))
+                  ; bytes := copy_bytes d (fst r_n) sz
+                                        (bytes (snd r_n)) |})
+         Else
+           (fst r_n + ` d0,
+            {| resvs := M.add (fst r_n) (` d0) (resvs (snd r_n))
+             ; bytes := bytes (snd r_n) |})).
+        simplify with monad laws.
+        finish honing.
+
+      simpl in *; intuition; rewrite ?H1;
+      (destruct (M.find d _) as [sz|] eqn:Heqe;
+       [ destruct (` d0 <=? sz) eqn:Heqe1;
+         simpl; rewrite ?Heqe1 |]); simpl.
+      - rewrite remove_add; reflexivity.
+      - reflexivity.
+      - apply F.add_m; auto.
+        apply F.Equal_mapsto_iff; split; intros.
+          simplify_maps.
+        simplify_maps; intuition.
+        subst.
+        apply F.find_mapsto_iff in H2.
+        congruence.
+      - rewrite copy_bytes_idem; assumption.
+      - rewrite N.min_l.
+          rewrite H0; reflexivity.
+        nomega.
+      - assumption.
+      - normalize.
+        apply_for_all; relational.
+        rewrite <- remove_add.
+        apply for_all_add_true; relational.
+          simplify_maps.
+        split.
+          apply for_all_remove; relational.
+        nomega.
+      - normalize.
+        apply_for_all; relational.
+        rewrite <- remove_add.
+        apply for_all_add_true; relational.
+          simplify_maps.
+        split.
+          apply for_all_remove; relational.
+          apply for_all_remove; relational.
+          eapply for_all_impl; eauto;
+          relational; nomega.
+        nomega.
+      - rewrite <- remove_add.
+        apply for_all_add_true; relational.
+          simplify_maps.
+        split.
+          apply for_all_remove; relational.
+          eapply for_all_impl; eauto;
+          relational; nomega.
+        nomega.
+    }
+    simpl in *; intuition; rewrite ?H1;
+    (destruct (M.find d _) as [sz|] eqn:Heqe;
+     [ destruct (` d0 <=? sz) eqn:Heqe1;
+       simpl; rewrite ?Heqe1 |]); simpl.
+    - normalize.
+      rewrite <- H1 in Heqe.
+      pose proof (allocations_no_overlap (proj2_sig r_o) Heqe).
+      apply P.for_all_iff; relational; intros.
+      simplify_maps.
+      rewrite <- H1 in H6.
+      specialize (H2 _ _ H6 H5).
+      nomega.
+    - normalize.
+      apply_for_all; relational.
+      apply for_all_remove; relational.
+      eapply for_all_impl; eauto;
+      relational; nomega.
+    - apply for_all_remove; relational.
+      eapply for_all_impl; eauto;
+      relational; nomega.
+  }
+
+  refine method peekS.
+  {
+    remove_dependency.
+    unfold peek.
+    simplify with monad laws; simpl.
+
+    refine pick val (Ifopt M.find d (bytes (snd r_n)) as v
+                     Then v
+                     Else Zero).
+    {
+      simplify with monad laws.
+      refine pick val r_n.
+        simplify with monad laws.
+        finish honing.
+      simpl in *; intuition.
+    }
+    simpl in *; intuition.
+    destruct (M.find d _) as [sz|] eqn:Heqe;
+    simpl; normalize.
+      rewrite H0 in H2.
+      pose proof (F.MapsTo_fun Heqe H2).
+      assumption.
+    rewrite H0 in H2.
+    apply F.find_mapsto_iff in H2.
+    congruence.
+  }
+
+  refine method pokeS.
+  {
+    remove_dependency.
+    unfold poke.
+    simplify with monad laws; simpl.
+
+    refine pick val (fst r_n,
+                     {| resvs := resvs (snd r_n)
+                      ; bytes := M.add d d0 (bytes (snd r_n)) |}).
+      simplify with monad laws.
+      finish honing.
+
+    simpl in *; intuition;
+    destruct (d <? fst r_n) eqn:Heqe; simpl; trivial;
+    rewrite H0; reflexivity.
+  }
+
+  refine method memcpyS.
+  {
+    remove_dependency.
+    unfold memcpy.
+    simplify with monad laws; simpl.
+
+    refine pick val (fst r_n,
+                     {| resvs := resvs (snd r_n)
+                      ; bytes := copy_bytes d d0 d1 (bytes (snd r_n)) |}).
+      simplify with monad laws.
+      finish honing.
+
+    simpl in *; intuition;
+    rewrite H0; reflexivity.
+  }
+
+  refine method memsetS.
+  {
+    remove_dependency.
+    unfold memset.
+    simplify with monad laws; simpl.
+
+    refine pick val
+       (fst r_n,
+        {| resvs := resvs (snd r_n)
+         ; bytes :=
+             P.update (bytes (snd r_n))
+                      (N.peano_rect (fun _ => M.t Word)
+                                    (bytes (snd r_n))
+                                    (fun i => M.add (d + i)%N d1) d0) |}).
+      simplify with monad laws.
+      finish honing.
+
+    simpl in *; intuition.
+    apply P.update_m; trivial.
+    induction d0 using N.peano_ind; simpl; trivial.
+    rewrite !N.peano_rect_succ.
+    apply F.add_m; trivial.
+  }
+
+  finish_SharpeningADT_WithoutDelegation.
+Defined.
+
+(*
+ /\
+          (* Every reservation is under the free marker *)
+          P.for_all (fun a sz => a + sz <=? fst nr) (resvs (snd nr))
+
+      - apply for_all_add_true; relational.
+          unfold not; intros.
+          destruct (proj1 (in_mapsto_iff _ _ _) H2).
+          rewrite <- H1 in H4.
+          pose proof (allocations_have_size (proj2_sig r_o) H4).
+          rewrite H1 in H4.
+          apply_for_all; relational.
+          nomega.
+        split; [|nomega].
+        eapply for_all_impl; eauto;
+        relational; nomega.
+*)
+
+End HeapCanonical.
