src/ByteString.v
@@ -1,24 +1,26 @@
 Require Import
   Fiat.ADT
   Fiat.ADTNotation
-  ByteString.Heap.
+  ByteString.Memory.
 
 (************************************************************************
  ** Semantics of the core Haskell ByteString data type in Fiat.        **
  ************************************************************************)
+
+Open Scope string_scope.
 
 Definition emptyS  := "empty".
 Definition consS   := "cons".
 Definition unconsS := "uncons".
 
 Definition ByteStringSpec := Def ADT {
-  rep := list Word8,
+  rep := list Word,
 
   Def Constructor0 emptyS : rep := ret []%list,,
 
-  Def Method1 consS (r : rep) (w : Word8) : rep * unit :=
+  Def Method1 consS (r : rep) (w : Word) : rep * unit :=
     ret (cons w r, tt),
-  Def Method0 unconsS (r : rep) : rep * (option Word8) :=
+  Def Method0 unconsS (r : rep) : rep * (option Word) :=
     ret (match r with
          | nil => (r, None)
          | cons x xs => (xs, Some x)
@@ -31,8 +33,8 @@ Definition ByteString := Rep ByteStringSpec.
 Definition empty : Comp ByteString :=
   Eval simpl in callCons ByteStringSpec emptyS.
 
-Definition cons (w : Word8) (bs : ByteString) : Comp ByteString :=
+Definition cons (w : Word) (bs : ByteString) : Comp ByteString :=
   Eval simpl in (p <- callMeth ByteStringSpec consS bs w; ret (fst p)).
 
-Definition uncons (bs : ByteString) : Comp (ByteString * option Word8) :=
+Definition uncons (bs : ByteString) : Comp (ByteString * option Word) :=
   Eval simpl in callMeth ByteStringSpec unconsS bs.
