src/ByteStringLib.v
@@ -2,31 +2,31 @@ Require Import
   Fiat.ADT
   Fiat.ADTNotation
   Fiat.Computation.FixComp
-  ByteString.Heap
+  ByteString.Memory
   ByteString.ByteString.
 
 (************************************************************************
  ** Semantics of the Haskell ByteString library in Fiat.               **
  ************************************************************************)
 
-Definition singleton_Spec (w : Word8) : Comp ByteString :=
+Definition singleton_Spec (w : Word) : Comp ByteString :=
   xs  <- callCons ByteStringSpec emptyS;
   res <- callMeth ByteStringSpec consS xs w;
   ret (fst res).
 
 (*
-Definition pack_Spec (xs : list Word8) : Comp ByteString :=
-Definition unpack_Spec (bs : ByteString) : Comp (ByteString * list Word8) :=
-Definition snoc (bs : ByteString) (w : Word8) : Comp (ByteString * unit) :=
+Definition pack_Spec (xs : list Word) : Comp ByteString :=
+Definition unpack_Spec (bs : ByteString) : Comp (ByteString * list Word) :=
+Definition snoc (bs : ByteString) (w : Word) : Comp (ByteString * unit) :=
 *)
 
 Import LeastFixedPointFun.
 
 Definition foldr_Spec {A} :
-  ByteString -> (Word8 -> A -> A) -> A -> Comp (ByteString * A) :=
-  LeastFixedPoint (fDom := [ByteString; Word8 -> A -> A; A])
+  ByteString -> (Word -> A -> A) -> A -> Comp (ByteString * A) :=
+  LeastFixedPoint (fDom := [ByteString; Word -> A -> A; A])
                   (fCod := ByteString * A)
-    (fun rec (bs : ByteString) (f : Word8 -> A -> A) (z : A) =>
+    (fun rec (bs : ByteString) (f : Word -> A -> A) (z : A) =>
        p <- uncons bs;
        Ifopt snd p as w
        Then bs' <- rec (fst p) f z;
@@ -35,9 +35,9 @@ Definition foldr_Spec {A} :
 
 (*
 append :: ByteString -> ByteString -> ByteString
-head :: ByteString -> Word8
-unsnoc :: ByteString -> Maybe (ByteString, Word8)
-last :: ByteString -> Word8
+head :: ByteString -> Word
+unsnoc :: ByteString -> Maybe (ByteString, Word)
+last :: ByteString -> Word
 *)
 
 Definition tail_Spec (bs : ByteString) : Comp (ByteString * bool) :=
@@ -50,70 +50,70 @@ Definition tail_Spec (bs : ByteString) : Comp (ByteString * bool) :=
 init :: ByteString -> ByteString
 null :: ByteString -> Bool
 length :: ByteString -> Int
-map :: (Word8 -> Word8) -> ByteString -> ByteString
+map :: (Word -> Word) -> ByteString -> ByteString
 reverse :: ByteString -> ByteString
-intersperse :: Word8 -> ByteString -> ByteString
+intersperse :: Word -> ByteString -> ByteString
 intercalate :: ByteString -> [ByteString] -> ByteString
 transpose :: [ByteString] -> [ByteString]
-foldl :: (a -> Word8 -> a) -> a -> ByteString -> a
-foldl' :: (a -> Word8 -> a) -> a -> ByteString -> a
-foldl1 :: (Word8 -> Word8 -> Word8) -> ByteString -> Word8
-foldl1' :: (Word8 -> Word8 -> Word8) -> ByteString -> Word8
-foldr :: (Word8 -> a -> a) -> a -> ByteString -> a
-foldr' :: (Word8 -> a -> a) -> a -> ByteString -> a
-foldr1 :: (Word8 -> Word8 -> Word8) -> ByteString -> Word8
-foldr1' :: (Word8 -> Word8 -> Word8) -> ByteString -> Word8
+foldl :: (a -> Word -> a) -> a -> ByteString -> a
+foldl' :: (a -> Word -> a) -> a -> ByteString -> a
+foldl1 :: (Word -> Word -> Word) -> ByteString -> Word
+foldl1' :: (Word -> Word -> Word) -> ByteString -> Word
+foldr :: (Word -> a -> a) -> a -> ByteString -> a
+foldr' :: (Word -> a -> a) -> a -> ByteString -> a
+foldr1 :: (Word -> Word -> Word) -> ByteString -> Word
+foldr1' :: (Word -> Word -> Word) -> ByteString -> Word
 concat :: [ByteString] -> ByteString
-concatMap :: (Word8 -> ByteString) -> ByteString -> ByteString
-any :: (Word8 -> Bool) -> ByteString -> Bool
-all :: (Word8 -> Bool) -> ByteString -> Bool
-maximum :: ByteString -> Word8
-minimum :: ByteString -> Word8
-scanl :: (Word8 -> Word8 -> Word8) -> Word8 -> ByteString -> ByteString
-scanl1 :: (Word8 -> Word8 -> Word8) -> ByteString -> ByteString
-scanr :: (Word8 -> Word8 -> Word8) -> Word8 -> ByteString -> ByteString
-scanr1 :: (Word8 -> Word8 -> Word8) -> ByteString -> ByteString
-mapAccumL :: (acc -> Word8 -> (acc, Word8)) -> acc -> ByteString -> (acc, ByteString)
-mapAccumR :: (acc -> Word8 -> (acc, Word8)) -> acc -> ByteString -> (acc, ByteString)
-replicate :: Int -> Word8 -> ByteString
-unfoldr :: (a -> Maybe (Word8, a)) -> a -> ByteString
-unfoldrN :: Int -> (a -> Maybe (Word8, a)) -> a -> (ByteString, Maybe a)
+concatMap :: (Word -> ByteString) -> ByteString -> ByteString
+any :: (Word -> Bool) -> ByteString -> Bool
+all :: (Word -> Bool) -> ByteString -> Bool
+maximum :: ByteString -> Word
+minimum :: ByteString -> Word
+scanl :: (Word -> Word -> Word) -> Word -> ByteString -> ByteString
+scanl1 :: (Word -> Word -> Word) -> ByteString -> ByteString
+scanr :: (Word -> Word -> Word) -> Word -> ByteString -> ByteString
+scanr1 :: (Word -> Word -> Word) -> ByteString -> ByteString
+mapAccumL :: (acc -> Word -> (acc, Word)) -> acc -> ByteString -> (acc, ByteString)
+mapAccumR :: (acc -> Word -> (acc, Word)) -> acc -> ByteString -> (acc, ByteString)
+replicate :: Int -> Word -> ByteString
+unfoldr :: (a -> Maybe (Word, a)) -> a -> ByteString
+unfoldrN :: Int -> (a -> Maybe (Word, a)) -> a -> (ByteString, Maybe a)
 take :: Int -> ByteString -> ByteString
 drop :: Int -> ByteString -> ByteString
 splitAt :: Int -> ByteString -> (ByteString, ByteString)
-takeWhile :: (Word8 -> Bool) -> ByteString -> ByteString
-dropWhile :: (Word8 -> Bool) -> ByteString -> ByteString
-span :: (Word8 -> Bool) -> ByteString -> (ByteString, ByteString)
-spanEnd :: (Word8 -> Bool) -> ByteString -> (ByteString, ByteString)
-break :: (Word8 -> Bool) -> ByteString -> (ByteString, ByteString)
-breakEnd :: (Word8 -> Bool) -> ByteString -> (ByteString, ByteString)
+takeWhile :: (Word -> Bool) -> ByteString -> ByteString
+dropWhile :: (Word -> Bool) -> ByteString -> ByteString
+span :: (Word -> Bool) -> ByteString -> (ByteString, ByteString)
+spanEnd :: (Word -> Bool) -> ByteString -> (ByteString, ByteString)
+break :: (Word -> Bool) -> ByteString -> (ByteString, ByteString)
+breakEnd :: (Word -> Bool) -> ByteString -> (ByteString, ByteString)
 group :: ByteString -> [ByteString]
-groupBy :: (Word8 -> Word8 -> Bool) -> ByteString -> [ByteString]
+groupBy :: (Word -> Word -> Bool) -> ByteString -> [ByteString]
 inits :: ByteString -> [ByteString]
 tails :: ByteString -> [ByteString]
-split :: Word8 -> ByteString -> [ByteString]
-splitWith :: (Word8 -> Bool) -> ByteString -> [ByteString]
+split :: Word -> ByteString -> [ByteString]
+splitWith :: (Word -> Bool) -> ByteString -> [ByteString]
 isPrefixOf :: ByteString -> ByteString -> Bool
 isSuffixOf :: ByteString -> ByteString -> Bool
 isInfixOf :: ByteString -> ByteString -> Bool
 breakSubstring :: ByteString -> ByteString -> (ByteString, ByteString)
 findSubstring :: ByteString -> ByteString -> Maybe Int
 findSubstrings :: ByteString -> ByteString -> [Int]
-elem :: Word8 -> ByteString -> Bool
-notElem :: Word8 -> ByteString -> Bool
-find :: (Word8 -> Bool) -> ByteString -> Maybe Word8
-filter :: (Word8 -> Bool) -> ByteString -> ByteString
-partition :: (Word8 -> Bool) -> ByteString -> (ByteString, ByteString)
-index :: ByteString -> Int -> Word8
-elemIndex :: Word8 -> ByteString -> Maybe Int
-elemIndices :: Word8 -> ByteString -> [Int]
-elemIndexEnd :: Word8 -> ByteString -> Maybe Int
-findIndex :: (Word8 -> Bool) -> ByteString -> Maybe Int
-findIndices :: (Word8 -> Bool) -> ByteString -> [Int]
-count :: Word8 -> ByteString -> Int
-zip :: ByteString -> ByteString -> [(Word8, Word8)]
-zipWith :: (Word8 -> Word8 -> a) -> ByteString -> ByteString -> [a]
-unzip :: [(Word8, Word8)] -> (ByteString, ByteString)
+elem :: Word -> ByteString -> Bool
+notElem :: Word -> ByteString -> Bool
+find :: (Word -> Bool) -> ByteString -> Maybe Word
+filter :: (Word -> Bool) -> ByteString -> ByteString
+partition :: (Word -> Bool) -> ByteString -> (ByteString, ByteString)
+index :: ByteString -> Int -> Word
+elemIndex :: Word -> ByteString -> Maybe Int
+elemIndices :: Word -> ByteString -> [Int]
+elemIndexEnd :: Word -> ByteString -> Maybe Int
+findIndex :: (Word -> Bool) -> ByteString -> Maybe Int
+findIndices :: (Word -> Bool) -> ByteString -> [Int]
+count :: Word -> ByteString -> Int
+zip :: ByteString -> ByteString -> [(Word, Word)]
+zipWith :: (Word -> Word -> a) -> ByteString -> ByteString -> [a]
+unzip :: [(Word, Word)] -> (ByteString, ByteString)
 sort :: ByteString -> ByteString
 copy :: ByteString -> ByteString
 *)
@@ -143,5 +143,5 @@ hPutStrLn :: Handle -> ByteString -> IO ()
 *)
 
 (*
-breakByte :: Word8 -> ByteString -> (ByteString, ByteString)
+breakByte :: Word -> ByteString -> (ByteString, ByteString)
 *)
