src/HeapEns.v
@@ -1,0 +1,446 @@
+Require Import
+  Fiat.ADT
+  Fiat.ADTNotation
+  ByteString.TupleEnsembles
+  ByteString.LibExt
+  ByteString.Nomega
+  ByteString.Decidable
+  ByteString.BindDep
+  ByteString.ADTInduction
+  ByteString.Same_set
+  ByteString.TupleEnsemblesFinite.
+
+Generalizable All Variables.
+
+Open Scope string_scope.
+
+Definition Word8 := Ascii.ascii.
+Definition Zero  := Ascii.zero.
+
+Record MemoryBlock := {
+  memSize : N;
+  memData : EMap N Word8
+}.
+
+Definition MemoryBlock_Same (x y : MemoryBlock) : Prop :=
+  memSize x = memSize y /\ Same (memData x) (memData y).
+
+Global Program Instance MemoryBlock_Proper :
+  Proper (eq ==> @Same _ _ ==> MemoryBlock_Same) Build_MemoryBlock.
+Obligation 1. relational; split; simpl; subst; auto. Qed.
+
+Ltac tsubst :=
+  repeat
+    match goal with
+    | [ H : (_, _) = (_, _) |- _ ] => inv H
+    | [ H : (_, _, _) = (_, _, _) |- _ ] => inv H
+    | [ H : (_, _, _, _) = (_, _, _, _) |- _ ] => inv H
+    | [ H : {| memSize := _
+             ; memData := _ |} =
+            {| memSize := _
+             ; memData := _ |} |- _ ] => inv H
+    end;
+  subst.
+
+Definition KeepKeys (P : N -> Prop) :
+  EMap N Word8 -> EMap N Word8 :=
+  Filter (fun k _ => P k).
+
+Definition ShiftKeys (orig_base : N) (new_base : N) :
+  EMap N Word8 -> EMap N Word8 :=
+  Map_set (fun p => (fst p - orig_base + new_base, snd p)).
+
+Definition FindFreeBlock (len : N) (heap : EMap N MemoryBlock) : Comp N :=
+  { addr : N | All (fun addr' blk' =>
+                      ~ overlaps addr' (memSize blk') addr len) heap }.
+
+Definition FindBlock (base : N) (heap : EMap N MemoryBlock) :
+  Comp (option MemoryBlock) :=
+  { blk : option MemoryBlock
+  | Ifopt blk as blk'
+    Then Lookup base blk' heap
+    Else ~ Member base heap }.
+
+Definition FindBlockThatFits (off len : N) (heap : EMap N MemoryBlock) :
+  Comp (option (N * MemoryBlock)) :=
+  { mres : option (N * MemoryBlock)
+  | match mres with
+    | Some (addr', blk') =>
+      Lookup addr' blk' heap /\ fits addr' (memSize blk') off len
+    | None =>
+      All (fun addr' blk' =>
+             ~ fits addr' (memSize blk') off len) heap
+    end }.
+
+Definition CopyBlock sblk soff dblk doff len :=
+  (* [s] is the source region to copy from *)
+  let s := KeepKeys (within soff len) (memData sblk) in
+  (* [d] is where the region will be copied *)
+  let d := KeepKeys (not ∘ within doff len) (memData dblk) in
+  Union _ d (ShiftKeys soff doff s).
+
+Definition emptyS   := "empty".
+Definition allocS   := "alloc".
+Definition reallocS := "realloc".
+Definition freeS    := "free".
+Definition peekS    := "peek".
+Definition pokeS    := "poke".
+Definition memcpyS  := "memcpy".
+Definition memsetS  := "memset".
+
+Definition HeapSpec := Def ADT {
+  (* Map of memory addresses to blocks, which contain another mapping from
+     offsets to initialized bytes. *)
+  rep := EMap N MemoryBlock,
+
+  Def Constructor0 emptyS : rep := ret Empty,,
+
+  (* Allocation returns the address for the newly allocated block.
+     NOTE: conditions such as out-of-memory are not handled here; the final
+     implementation must decide how to handle this operationally, such as by
+     throwing an exception. It remains a further research question how to
+     specify error handling at this level, when certain errors -- such as
+     exhausting memory -- do not belong here, since a mathematical machine has
+     no such limits. *)
+  Def Method1 allocS (r : rep) (len : N | 0 < len) : rep * N :=
+    addr <- FindFreeBlock (` len) r;
+    ret (Update addr {| memSize := ` len
+                      ; memData := Empty |} r, addr),
+
+  (* Freeing an unallocated block is a no-op. *)
+  Def Method1 freeS (r : rep) (addr : N) : rep * unit :=
+    ret (Remove addr r, tt),
+
+  (* Realloc is not required to reuse the same block. If the address does not
+     identify an allociated region, a new memory block is returned without any
+     bytes moved. If a block did exist previously, as many bytes as possible
+     are copied to the new block. *)
+  Def Method2 reallocS (r : rep) (addr : N) (len : N | 0 < len) : rep * N :=
+    present <- FindBlock addr r;
+    naddr   <- FindFreeBlock (` len) (Remove addr r);
+    ret (
+      Ifopt present as blk
+      Then Update naddr {| memSize := ` len
+                         ; memData := Filter (fun pos _ => pos < ` len)
+                                             (memData blk) |} (Remove addr r)
+      Else Update naddr {| memSize := ` len
+                         ; memData := Empty |} r,
+      naddr),
+
+  (* Peeking an unallocated address allows anydefault value to be returned. *)
+  Def Method1 peekS (r : rep) (addr : N) : rep * Word8 :=
+    mres <- FindBlockThatFits addr 1 r;
+    p <- { p : Word8
+         | forall v base' blk', mres = Some (base', blk')
+             -> Lookup (addr - base') v (memData blk')
+             -> p = v };
+    ret (r, p),
+
+  (* Poking an unallocated address is a no-op. *)
+  Def Method2 pokeS (r : rep) (addr : N) (w : Word8) : rep * unit :=
+    ret (Map (fun base blk =>
+                Ifdec within base (memSize blk) addr
+                Then {| memSize := memSize blk
+                      ; memData := Update (addr - base) w (memData blk) |}
+                Else blk) r, tt),
+
+  (* Data may only be copied from one allocated block to another (or within
+     the same block), and the region must fit within both source and
+     destination. Otherwise, the operation is a no-op. *)
+  Def Method3 memcpyS (r : rep) (addr1 : N) (addr2 : N) (len : N) :
+    rep * unit :=
+      Ifdec 0 < len
+      Then (
+        ms <- FindBlockThatFits addr1 len r;
+        ret (Ifopt ms as s
+             Then
+               Map (fun daddr dblk =>
+                 Ifdec fits daddr (memSize dblk) addr2 len
+                 Then {| memSize := memSize dblk
+                       ; memData :=
+                           let soff := addr1 - fst s in
+                           let doff := addr2 - daddr in
+                           CopyBlock (snd s) soff dblk doff len |}
+                 Else dblk) r
+             Else r, tt))
+      Else ret (r, tt),
+
+  (* Any attempt to memset bytes outside of an allocated block is a no-op. *)
+  Def Method3 memsetS (r : rep) (addr : N) (len : N) (w : Word8) :
+    rep * unit :=
+    ret (Map (fun base blk =>
+                Ifdec fits base (memSize blk) addr len
+                Then {| memSize := memSize blk
+                      ; memData := Define (within (addr - base) len) w
+                                          (memData blk) |}
+                Else blk) r, tt)
+
+}%ADTParsing.
+
+Definition empty : Comp (Rep HeapSpec) :=
+  Eval simpl in callCons HeapSpec emptyS.
+
+Definition alloc (r : Rep HeapSpec) (len : N | 0 < len) :
+  Comp (Rep HeapSpec * N) :=
+  Eval simpl in callMeth HeapSpec allocS r len.
+
+Definition free (r : Rep HeapSpec) (addr : N) :
+  Comp (Rep HeapSpec * unit) :=
+  Eval simpl in callMeth HeapSpec freeS r addr.
+
+Definition realloc (r : Rep HeapSpec) (addr : N) (len : N | 0 < len) :
+  Comp (Rep HeapSpec * N) :=
+  Eval simpl in callMeth HeapSpec reallocS r addr len.
+
+Definition peek (r : Rep HeapSpec) (addr : N) :
+  Comp (Rep HeapSpec * Word8) :=
+  Eval simpl in callMeth HeapSpec peekS r addr.
+
+Definition poke (r : Rep HeapSpec) (addr : N) (w : Word8) :
+  Comp (Rep HeapSpec * unit) :=
+  Eval simpl in callMeth HeapSpec pokeS r addr w.
+
+Definition memcpy (r : Rep HeapSpec) (addr : N) (addr2 : N) (len : N) :
+  Comp (Rep HeapSpec * unit) :=
+  Eval simpl in callMeth HeapSpec memcpyS r addr addr2 len.
+
+Definition memset (r : Rep HeapSpec) (addr : N) (len : N) (w : Word8) :
+  Comp (Rep HeapSpec * unit) :=
+  Eval simpl in callMeth HeapSpec memsetS r addr len w.
+
+(**
+ ** Theorems related to the Heap specification.
+ **)
+
+Ltac inspect :=
+  repeat (unfold KeepKeys, ShiftKeys, CopyBlock,
+                 FindFreeBlock, FindBlock, FindBlockThatFits in *;
+          destruct_computations; simpl in *;
+          repeat teardown; tsubst; simpl in *;
+          decisions; eauto with sets;
+          try congruence).
+
+Ltac complete IHfromADT :=
+  inspect;
+  try match goal with
+    [ H : (?X =? ?Y) = true |- _ ] => apply N.eqb_eq in H; subst
+  end;
+  try (eapply IHfromADT; eassumption);
+  try solve [ eapply IHfromADT; try eassumption; inspect
+            | try eapply IHfromADT; eassumption
+            | inspect;
+              try (unfold fits, within in *; inspect; nomega);
+              eapply IHfromADT; try eassumption; inspect
+            | discriminate ].
+
+Theorem allocations_have_size : forall r : Rep HeapSpec, fromADT _ r ->
+  forall addr blk, Lookup addr blk r -> 0 < memSize blk.
+Proof.
+  intros.
+  generalize dependent blk.
+  generalize dependent addr.
+  ADT induction r; [inversion H0|..]; complete IHfromADT.
+Qed.
+
+Theorem allocations_correct_offsets : forall r : Rep HeapSpec, fromADT _ r ->
+  forall addr blk, Lookup addr blk r ->
+    All (fun off _ => off < memSize blk) (memData blk).
+Proof.
+  intros.
+  generalize dependent blk.
+  generalize dependent addr.
+  ADT induction r; [inversion H0|..]; intros ???;
+  complete IHfromADT.
+Qed.
+
+Ltac match_sizes H IHfromADT :=
+  match goal with
+  | [ H1 : Lookup ?A ?X ?R, H2 : Lookup ?B ?Y ?R |- _ ] =>
+    specialize (IHfromADT _ _
+                  H1 (allocations_have_size H _ _ H1) _
+                  H2 (allocations_have_size H _ _ H2)); subst
+  end; inspect; auto.
+
+Ltac match_sizes_r H IHfromADT :=
+  match goal with
+  | [ H1 : Lookup ?A ?X ?R, H2 : Lookup ?B ?Y ?R |- _ ] =>
+    try rewrite <- (IHfromADT _ _
+                      H1 (allocations_have_size H _ _ H1) _
+                      H2 (allocations_have_size H _ _ H2)) in *
+  end; inspect; auto.
+
+Ltac check_overlaps :=
+  match goal with
+    [ H1 : All (fun addr' blk' => ~ overlaps addr' (memSize blk') ?XA ?XL)
+               (Remove ?YA ?R),
+      H2 : ?XA <> ?YA,
+      H3 : 0 < ?XL,
+      H4 : Lookup ?XA ?B ?R,
+      H5 : 0 < memSize ?B |- _ ] =>
+    eapply All_Remove_Lookup_inv with (a':=XA) in H1; eauto;
+    contradiction (overlaps_irr XA H5 H3)
+  end.
+
+Theorem allocations_functional : forall r : Rep HeapSpec, fromADT _ r ->
+  Functional r.
+Proof.
+  unfold Functional; intros.
+  pose proof (allocations_have_size H _ _ H0).
+  pose proof (allocations_have_size H _ _ H1).
+  generalize dependent blk2.
+  generalize dependent blk1.
+  generalize dependent addr.
+  ADT induction r; [inversion H0|..]; inspect;
+  try solve [ match_sizes H IHfromADT ];
+  try discriminate;
+  check_overlaps.
+Qed.
+
+Theorem all_block_maps_are_functional : forall r : Rep HeapSpec, fromADT _ r ->
+  All (fun _ blk => Functional (memData blk)) r.
+Proof.
+  unfold All, Functional; intros.
+  generalize dependent b.
+  generalize dependent a.
+  generalize dependent blk1.
+  generalize dependent blk2.
+  generalize dependent addr.
+  ADT induction r; inspect.
+  - unfold compose in *; nomega.
+  - unfold compose in *; nomega.
+  - apply N.add_cancel_r in H9.
+    apply Nsub_eq in H9.
+    + subst.
+      clear H4.
+      eapply IHfromADT; eauto.
+    + nomega.
+    + nomega.
+  - inv H3; inv H4; congruence.
+Qed.
+
+Corollary allocations_functional_r : forall r : Rep HeapSpec, fromADT _ r ->
+  forall addr1 blk, Lookup addr1 blk r ->
+  forall addr2, ~ Member addr2 r -> addr1 <> addr2.
+Proof.
+  unfold not; intros; subst; ADT induction r;
+  contradiction H1;
+  exists blk; assumption.
+Qed.
+
+Ltac lookup_uid H :=
+  match goal with
+  | [ H1 : Lookup ?A ?X ?R, H2 : Lookup ?A ?Y ?R |- _ ] =>
+    pose proof (allocations_functional H _ _ H1 _ H2); subst
+  end; inspect; auto.
+
+Theorem allocations_no_overlap : forall r : Rep HeapSpec, fromADT _ r ->
+  forall addr1 blk1, Lookup addr1 blk1 r ->
+  forall addr2 blk2, Lookup addr2 blk2 r
+    -> addr1 <> addr2
+    -> ~ overlaps addr1 (memSize blk1) addr2 (memSize blk2).
+Proof.
+  intros.
+  pose proof (allocations_have_size H _ _ H0).
+  pose proof (allocations_have_size H _ _ H1).
+  generalize dependent blk2.
+  generalize dependent addr2.
+  generalize dependent blk1.
+  generalize dependent addr1.
+  ADT induction r; [inversion H0|..]; complete IHfromADT;
+  try lookup_uid H; eapply All_Remove_Lookup_inv in H0'; eauto;
+  try nomega; eapply allocations_functional_r in H0; eauto.
+Qed.
+
+Corollary allocations_unique_fits : forall r : Rep HeapSpec, fromADT _ r ->
+  forall base blk addr len,
+    Lookup base blk r ->
+    fits base (memSize blk) addr len ->
+    Unique (fun a' b' => fits_bool a' (memSize b') addr len) base r.
+Proof.
+  unfold Unique; intros; intros ???.
+  apply Lookup_Remove_inv in H2; destruct H2.
+  pose proof (allocations_no_overlap H _ H3 _ H0 H2); nomega.
+Qed.
+
+Corollary allocations_unique_within : forall r : Rep HeapSpec, fromADT _ r ->
+  forall base blk addr,
+    Lookup base blk r ->
+    within base (memSize blk) addr ->
+    Unique (fun a' b' => within_bool a' (memSize b') addr) base r.
+Proof.
+  unfold Unique; intros; intros ???.
+  apply Lookup_Remove_inv in H2; destruct H2.
+  pose proof (allocations_no_overlap H _ H3 _ H0 H2); nomega.
+Qed.
+
+Corollary find_partitions_a_singleton : forall r : Rep HeapSpec, fromADT _ r ->
+  forall addr base blk,
+    Lookup base blk r
+      -> within base (memSize blk) addr
+      -> Same (Filter (fun a b => within a (memSize b) addr) r)
+              (Single base blk).
+Proof.
+  intros.
+  pose proof (allocations_no_overlap H _ H0).
+  pose proof (allocations_functional H _ _ H0).
+  split; intros; inspect;
+  destruct (N.eq_dec base a); subst; auto.
+  - specialize (H2 _ _ H5 n); nomega.
+  - specialize (H3 _ H5); nomega.
+  - specialize (H2 _ _ H5 n); nomega.
+Qed.
+
+Corollary allocations_disjoint : forall r : Rep HeapSpec, fromADT _ r ->
+  forall addr blk, Lookup addr blk r
+    -> forall pos, within addr (memSize blk) pos
+    -> forall addr' blk', Lookup addr' blk' r
+         -> addr <> addr'
+         -> ~ within addr' (memSize blk') pos.
+Proof. intros; pose proof (allocations_no_overlap H _ H0 _ H2 H3); nomega. Qed.
+
+Theorem heap_is_finite : forall r : Rep HeapSpec, fromADT _ r -> Finite _ r.
+Proof. intros; ADT induction r; inspect; finite_preservation; nomega. Qed.
+
+Lemma added : forall b e,
+  b <= e -> Same_set _ (fun x : N => b <= x < N.succ e)
+                       (Add _ (fun x : N => b <= x < e) e).
+Proof.
+  unfold Same_set, Included, Add, Ensembles.In.
+  split; intros.
+    destruct (N.eq_dec x e); subst.
+      right; constructor.
+    left; unfold Ensembles.In in *; nomega.
+  inv H0; unfold Ensembles.In in *;
+  destruct H1; nomega.
+Qed.
+
+Lemma not_added : forall b e,
+  ~ b <= e -> Same_set _ (fun x : N => b <= x < N.succ e)
+                         (fun x : N => b <= x < e).
+Proof. unfold Same_set, Included, Add, Ensembles.In; nomega. Qed.
+
+Lemma N_Finite : forall b e, Finite N (fun x : N => b <= x < e).
+Proof.
+  intros.
+  induction e using N.peano_ind; intros.
+    eapply Finite_downward_closed; eauto with sets.
+    unfold Included, Ensembles.In; nomega.
+  destruct (N.le_decidable b e).
+    rewrite added; trivial.
+    constructor; trivial.
+    unfold Ensembles.In; nomega.
+  rewrite not_added; trivial.
+Qed.
+
+Hint Extern 5 (Finite N (within _ _)) => apply N_Finite.
+
+Theorem all_blocks_are_finite : forall r : Rep HeapSpec, fromADT _ r ->
+  All (fun _ blk => Finite _ (memData blk)) r.
+Proof.
+  unfold All; intros.
+  generalize dependent b.
+  generalize dependent a.
+  ADT induction r; inspect;
+  finite_preservation;
+  eauto; nomega.
+Qed.
