src/Memory.v
@@ -1,0 +1,8 @@
+Require Import
+  Coq.NArith.NArith
+  Coq.Strings.Ascii.
+
+Definition Ptr  := N.
+Definition Size := N.
+Definition Word := Ascii.ascii.
+Definition Zero := Ascii.zero.
